Kip/Ext.lean
@@ -1,0 +1,45 @@
+set_option autoImplicit false
+-- set_option linter.unusedVariables false
+
+-- class inductive Ext.{u} {T: Type u} (eval: T → T → T): T → T → Prop
+--   | ext {f g: T} (extEq: ∀x, Ext eval (eval f x) (eval g x)): Ext eval f g
+inductive Ext.{u} {T: Type u} (eval: T → T → T): T → T → Prop
+  | ext {f g: T} (extEq: ∀x, eval f x = eval g x): Ext eval f g
+namespace Ext
+  universe u
+  variable {T: Type u} (eval: T → T → T) (f g h: T)
+
+  theorem refl: Ext eval f f := ext fun _ => rfl
+  theorem symm: Ext eval f g → Ext eval g f
+    | ext e => ext fun x =>
+      match f, g, e x with
+      | _, _, rfl => rfl
+end Ext
+
+/-
+inductive Term.{u} (Var: Type u) where
+  | var (x: Var)
+  | lam (binder: Var) (predicate: Term Var)
+  | app (function argument: Term Var)
+namespace Term
+
+universe u
+variable {Var: Type u}
+
+instance: Coe Var (Term Var) where coe := var
+infixr:25 " ↦ " => lam
+instance: CoeFun (Term Var) (fun _ => Term Var → Term Var) where coe := app
+
+
+
+end Term
+-/
+
+-- abbrev ExtConst (t: Term) := Ext (fun _ _ => t)
+-- theorem refl (t: Term): ExtConst t t t := ext fun _ => refl t
+
+-- theorem reflUniq {eval eval': Term → Term → Term}
+--   : (∀x, Ext eval x x) → (∀x, Ext eval' x x) → ∀ f x, eval f x = eval' f x
+--   | h, h', f, x =>
+--     match h f, h' f with
+--     | ext k, ext k' => _
