Kip/Lam.lean
@@ -1,0 +1,140 @@
+/-
+- [λ](https://en.wikipedia.org/wiki/Lambda_calculus_definition)
+- [η](https://math.stackexchange.com/a/836124)
+- [substitution vs application](https://cs.stackexchange.com/questions/69790/difference-between-beta-reduction-and-substitution)
+- https://math.stackexchange.com/questions/1832272/categorical-semantics-explained-what-is-an-interpretation
+- [capture-avoiding substitution](https://en.wikipedia.org/wiki/Lambda_calculus#Capture-avoiding_substitutions)
+- [efficient term rewrite](https://math.stackexchange.com/a/4090017)
+
+All equivalences (α,β,η) are guided by extensionality.
+-/
+import Kip.Prelude
+set_option autoImplicit false
+-- set_option linter.unusedVariables false
+
+inductive Term.{u} (Var: Type u) where
+  | var (x: Var)
+  | lam (binder: Var) (predicate: Term Var)
+  | app (function argument: Term Var)
+namespace Term
+
+universe u
+variable {Var: Type u}
+
+instance: Coe Var (Term Var) where coe := var
+infixr:25 " ↦ " => lam
+instance: CoeFun (Term Var) (fun _ => Term Var → Term Var) where coe := app
+
+inductive free (x: Var): Term Var → Prop
+  | var: free x x
+  | lam {y: Var} {t: Term Var}: x ≠ y → free x t → free x (y ↦ t)
+  | appFun {f a: Term Var}: free x f → free x (f a)
+  | appArg {f a: Term Var}: free x a → free x (f a)
+instance: Membership Var (Term Var) where mem := free
+
+-- theorem free_var_iff_eq {x y: Var}: x ∈ var y ↔ x = y :=
+--   ⟨fun | .var => rfl, fun | rfl => .var⟩
+
+variable [DecidableEq Var]
+
+instance freeDec (x: Var): (t: Term Var) → Decidable (x ∈ t)
+  | var y =>
+    if h: x = y then isTrue (h ▸ .var) else isFalse fun | .var => h rfl
+  | lam y t =>
+    if h: x = y then isFalse fun | .lam hn _ => hn h else
+    match freeDec x t with
+    | isTrue h' => isTrue (.lam h h')
+    | isFalse h' => isFalse fun | .lam _ h => h' h
+  | app f a => 
+    match freeDec x f, freeDec x a with
+    | isTrue hf, _ => isTrue (.appFun hf)
+    | _, isTrue ha => isTrue (.appArg ha)
+    | isFalse hnf, isFalse hna => isFalse fun
+      | .appFun hf => hnf hf
+      | .appArg ha => hna ha
+
+/-- Should be a `Prop`, but Lean4 has its limits. -/
+class inductive substitutable (x: Var) (t: Term Var): Term Var → Prop
+  | var (y: Var): substitutable x t y
+  | lamBound (A: Term Var): substitutable x t (x ↦ A)
+  | lamFree {y: Var} {A: Term Var} -- `x ≠ y` is unnecessary
+    : y ∉ t → substitutable x t A → substitutable x t (y ↦ A)
+  | app {f a: Term Var}
+    : substitutable x t f → substitutable x t a → substitutable x t (f a)
+
+/-- Capture-avoiding substitution: `A[x←t]`. -/
+def subst (x: Var) (t: Term Var)
+  : (A: Term Var) → [precond: substitutable x t A] → Term Var
+  | A@(var y), _ => if x = y then t else A
+  | A@(y ↦ B), h => if e: x = y then A else
+    have: substitutable x t B := match h, e with | .lamFree _ h, _ => h
+    y ↦ subst x t B
+  | app f a, h =>
+    have: substitutable x t f := have .app hf _ := h; hf
+    have: substitutable x t a := have .app _ ha := h; ha
+    (subst x t f) (subst x t a)
+
+-- @[inherit_doc subst]
+-- macro A:term noWs "[" x:ident "←" t:term "]'" h:term:max : term =>
+--   `(subst $x $t $A (precond := $h))
+@[inherit_doc subst]
+macro:max A:term noWs "[" x:ident "←" t:term "]" : term => `(subst $x $t $A)
+example {x: Var} {t A: Term Var} [substitutable x t A]: A[x←t] = subst x t A := rfl
+
+-- @[inherit_doc subst]
+-- macro:max A:term noWs "[" x:ident "←" t:term "]" : term => `(subst <| by first
+--   | exact subst_self.precond $x $A
+--   | fail "Failed to prove that the substitution avoids capture. Try:
+-- - `have`-expressions to prove that the substitution avoids capture, or
+-- - the `A[x←t]'h` notation, where `h` is a proof that the substitution avoids capture."
+-- )
+
+-- @[inherit_doc subst]
+-- syntax:max term noWs "[" withoutPosition(term "←" term) "]" : term
+-- macro_rules | `($A[$x←$x]) => `(subst (subst_self.precond $x $A))
+
+section variable (A: Term Var) (x: Var)
+local instance: substitutable x (var x) A := sorry
+theorem subst_self: (A: Term Var) → A[x←x] = A
+  | var y => if e: x = y then trans (if_pos e) (congrArg var e) else if_neg e
+  | y ↦ B => if e: x = y then dif_pos e else
+    have hB := subst_self B
+    trans (if_neg e) (congrArg (y ↦ .) hB)
+  | app f a =>
+    have hf := subst_self f
+    have ha := subst_self a
+    congr (congrArg app hf) ha
+end
+
+section variable {x: Var} {A: Term Var} (t: Term Var) (nonfree: x ∉ A)
+local instance: substitutable x t A := sorry
+theorem subst_nonfree {x: Var} {A: Term Var} (nonfree: x ∉ A): A[x←t] = A :=
+  match A with
+  | var y => if_neg fun | rfl => nonfree .var
+  | y ↦ B => if e: x = y then dif_pos e else
+    have hB := subst_nonfree (nonfree ∘ .lam e)
+    trans (if_neg e) (congrArg (y ↦ .) hB)
+  | app f a =>
+    have hf := subst_nonfree (nonfree ∘ .appFun)
+    have ha := subst_nonfree (nonfree ∘ .appArg)
+    congr (congrArg app hf) ha
+end
+
+protected abbrev closed (A: Term Var): Prop := ∀ x: Var, x ∉ A
+
+section variable {A: Term Var} (closed: A.closed) (x: Var) (t: Term Var)
+local instance: substitutable x t A := sorry
+theorem subst_closed: A[x←t] = A := subst_nonfree t (closed x)
+end
+
+end Term
+
+/-
+Two caveats of α-conversion.
+- `λx.λx.x` could be α-converted into `λy.λx.x` but not `λy.λx.y`.
+- `x with y` in `λx.λy.x`, we get `λy.λy.y`, which is not at all the same
+-/
+
+#check {x: Nat // x < 3 }
+example (l: List Nat): l[0]'sorry = 0 := sorry
+#check And
